examples/increment/IncHeader.v
@@ -1,0 +1,5 @@
+Require Import CRIS.
+
+Module IncName.
+  Definition Inc : string := "Inc.inc".
+End IncName.
