examples/increment/IncI.v
@@ -1,0 +1,8 @@
+(* Require Import CRIS.
+Require Import ImpPrelude.
+
+Module IncI. Section IncI.
+  Definition inc : val → itree pmodE val :=
+    λ args,
+      '(b, ofs) : mblock * ptrofs <- (pargs [Tptr] [args])?;;
+      Ret (Vptr b ofs). *)
